# My first TTL file
# SJP 11 Feb 2020
# Author: Stephen J Pratt
# Contact: stephen.pratt@awe.gov.au
#
# This vocabulary describes information objects relating to plant health surveillance using RDF (Resource Description Framework).
# It is written (serialised) in Terse RDF Triple Language (Turtle).
# 
# Plant health surveillance involves field observations 
#
# See: https://en.wikipedia.org/wiki/Resource_Description_Framework
# 

# Prefix for this namespace is 'phs', for Plant Health Surveillance
#TODO # Ideally, this should be altered to linked.data.gov.au for persistence 
@prefix phs: <https://example.org/PlantHealthSurveillanceOntology#> .
@prefix ffly: <https://example.org/def/fruitfly> .

@prefix foaf: <http://xmlns.com/foaf/0.1/> .
@prefix rdf: <http://www.w3.org/1999/02/22-rdf-syntax-ns#> .
@prefix rdfs: <http://www.w3.org/2000/01/rdf-schema#> .
@prefix skos: <http://www.w3.org/2004/02/skos/core#> .
@prefix dcterms: <http://purl.org/dc/terms/> .           # DCMI gently encourages use of the /terms/ namespace (over /elements/1.1/)
@prefix dwc: <http://rs.tdwg.org/dwc/terms/> .
@prefix tgn: <http://vocab.getty.edu/tgn/> .         # Getty Thesaurus of Geographic Names
@prefix sdo: <https://schema.org/> .
@prefix sosa: <http://www.w3.org/ns/sosa/> .
@prefix ssn: <http://www.w3.org/ns/ssn/> .
@prefix owl: <http://www.w3.org/2002/07/owl#> .
@prefix rdf: <http://www.w3.org/1999/02/22-rdf-syntax-ns#> .
@prefix rdfs: <http://www.w3.org/2000/01/rdf-schema#> .
@prefix vann: <http://purl.org/vocab/vann/> .
@prefix xml: <http://www.w3.org/XML/1998/namespace> .
@prefix xsd: <http://www.w3.org/2001/XMLSchema#> .
# See https://prefix.cc/ for rdf namespace lookups

# Ontology declaration
<https://example.org/PlantHealthSurveillanceOntology>
  a owl:Ontology ;
  rdfs:label "Plant Health Surveillance Ontology"@en ;
  rdfs:comment "An ontology about surveillance to determine plant health, such as fruit fly trapping."@en ;
  dcterms:created "2020-02-11"^^xsd:date ;
  dcterms:modified "2020-03-18"^^xsd:date ;
  dcterms:creator [
    a owl:NamedIndividual ;
    a sdo:Person ;
    sdo:email <mailto:stephen.pratt@awe.gov.au> ;
    sdo:jobTitle "Project Manager: Implementation of Plant Health Surveillance Data Store" ;
    sdo:affiliation <https://www.csiro.au.com> ;
    sdo:name "Stephen J. Pratt" ;
  ] ;
  dcterms:contributor 
    <http://orcid.org/0000-0002-8742-7730> , 
    <https://orcid.org/0000-0002-3884-3420> ;
  owl:versionIRI <https://example.org/PlantHealthSurveillanceOntology/0.1> ;
  owl:versionInfo "Initial version" ;
  sdo:codeRepository <https://github.com/F3RR3T/PlantHealthSurveillanceOntology> ;
  vann:preferredNamespacePrefix "phs" ;
.

<https://www.awe.gov.au>  # to be replaced with a more persistent org URI when we get it from AGOR / Linked Data WG
  a owl:NamedIndividual ;
  a sdo:Organization ;
  sdo:name "Department of Agriculture, Water and the Environment" ;
  sdo:url <https://www.awe.gov.au> ;
.
<https://orcid.org/0000-0002-3884-3420>
  a owl:NamedIndividual ;
  a sdo:Person ;
  sdo:email <mailto:simon.cox@surroundaustralia.com> ;
  sdo:jobTitle "Research Scientist" ;
  sdo:affiliation <https://www.csiro.au.com> ;
  sdo:name "Simon J.D. Cox" ;
.

<https://www.csiro.au.com>
  a owl:NamedIndividual ;
  a sdo:Organization ;
  sdo:name "CSIRO" ;
  sdo:url <https://www.csiro.au.com> ;
.

<http://orcid.org/0000-0002-8742-7730>
  a owl:NamedIndividual ;
  a sdo:Person ;
  sdo:email <mailto:nicholas.car@surroundaustralia.com> ;
  sdo:jobTitle "Data Systems Architect" ;
  sdo:affiliation <https://surroundaustralia.com> ;
  sdo:name "Nicholas J. Car" ;
.

<https://surroundaustralia.com>
  a owl:NamedIndividual ;
  a sdo:Organization ;
  sdo:name "SURROUND Australia Pty Ltd" ;
  sdo:url <https://surroundaustralia.com> ;
.

#Classes
phs:Trap
  a owl:Class ;
  rdfs:subClassOf sosa:Sampler ;
  rdfs:label "Trap" ;
  rdfs:comment "A device that catches or collects organisms or evidence of them" ;
.
phs:InsectTrap
  a owl:Class ;
  rdfs:label "A device that catches or collects insects" ;
  rdfs:seeAlso <http://dbpedia.org/resource/Insect_trap> ;
  rdfs:subClassOf phs:Trap ;
  rdfs:label "Insect Trap" ;
  rdfs:comment "A device that catches or collects insects" ;
.
phs:Lure
  a owl:Class ;
  rdfs:label "Lure" ;
  rdfs:comment "An attractant that may be placed in an InsectTrap" ;
.
phs:Stratum
  a owl:Class ;
  rdfs:label "Stratum" ;
  rdfs:comment "Thing or material on which a pest is searched for or found upon. A superclass for host or substrate." ;
.
phs:Substrate 
  a owl:Class ;
  rdfs:subClassOf phs:Stratum ;
  rdfs:label "Substrate" ;
  rdfs:comment "A non-living thing on which a pest may be found." ;
.
phs:Host
  a owl:Class ;
  rdfs:subClassOf phs:Stratum ;
  rdfs:subClassOf dwc:Taxon ;
  rdfs:label "Host" ;
  rdfs:comment "A plant on (or in) which a pest may be found." ;
.
phs:TrapType 
  a owl:Class ;
  rdfs:subClassOf skos:Concept ;
  rdfs:label "Trap Type" ;
.
#Properties
phs:trapType
  a owl:ObjectProperty ;
  rdfs:domain phs:InsectTrap ;
  rdfs:range phs:TrapType ;
  rdfs:comment "should we declarea range here for allowed types?" ;
  rdfs:comment "The make or model of a trap" ;
.
# Might be better to create the term 'TrapModel' for commercial names of trap.
# That would leave 'TrapType' for ['Light trap', 'Pitfall trap', 'Adhesive trap',
#   'Flying insect trap', ...]
# Or do we use the RANGE to define allowed values?
phs:lureType
  a owl:ObjectProperty ;
  rdfs:domain phs:Lure ;
  rdfs:range skos:Concept ;  # an item from a controlled vocabaulary - placeholder until a LureType specialization is defined
.
# Individuals
ffly:TrapTypes
  a skos:Collection ;
  rdfs:label "Collection of allowed names for trap types" ;
  skos:member ffly:Lyndfield ;
  skos:member ffly:Peyton;
  skos:member ffly:AnotherOne;
.
# I have introduced the ffly namespace specifically for fruit fly terms
ffly:Lyndfield
  a phs:TrapType ;
.
ffly:Peyton
  a phs:TrapType ;
.
ffly:AnotherOne
  a phs:TrapType ;
.
# Make a Canonical collection of lure type
# TODO - Alias list to collect wild-type variations of accepted terms
# TaxaaS (Taxonomy as a Service) has been depricated by the dept, so I'll use it 
# to refer to the API of any taxonomic reference system (GBIF, ALA, 'TRS').


#TARGET PEST
phs:TargetPest 
  a dwc:Taxon ;
  owl:equivalentClass dwc:Taxon ;
  rdfs:comment "The pest taxon that is is the subject of surveillance. Can have more than one target." ;
.
phs:targetTaxonomicReferenceSource
  a dcterms:Dataset ;
  rdfs:comment "The name of the taxonomic reference system used for this target" ;
  rdfs:comment "Placeholder Class relationship" ;
.
phs:targetTaxonID
  a phs:TargetPest ;
  rdfs:comment "Identifier for taxon proprties (including the following) of the Target Pest" ;
  owl:equivalentProperty dwc:taxonID ;
  rdfs:comment "Automatically populated by TaxaaS. Unsure whether we need taxonID AND taxonConceptID" ;
.
phs:targetTaxonConceptID
  a phs:TargetPest ;
  rdfs:comment "Identifier for taxonomic CONCEPT (not nomenclature) of the Target Pest" ;
  owl:equivalentProperty dwc:taxonConceptID ;
  rdfs:comment "Automatically populated by TaxaaS. Unsure whether we need taxonID AND taxonConceptID" ;
.
phs:targetCommonName
  a phs:TargetPest ;
  rdfs:comment "The vernacular (common) name for the Target Pest" ;
  owl:equivalentProperty dwc:vernacularName ;
  rdfs:comment "I'd prefer to use targetVernacularName and then do a 'common sameas vernacular'" ;
.
phs:targetScientificName
  a phs:TargetPest ;
  owl:equivalentProperty dwc:scientificName ;
  rdfs:comment "The scientific name of the target pest" ;
  rdfs:comment "I changed this from taxonName to align with DwC'" ;
.
# Other properties such as rank, parent taxon can be inferred from TaxaaS.

# HOST
phs:Host
  a dwc:Taxon ;
  owl:equivalentClass dwc:Taxon ;
  rdfs:comment "The host taxon that is is the subject of surveillance. Can have more than one host." ;
.
phs:hostTaxonomicReferenceSource
  a dcterms:Dataset ;
  rdfs:comment "The name of the taxonomic reference system used for this host" ;
  rdfs:comment "Placeholder Class relationship" ;
.
phs:hostTaxonID
  a phs:Host ;
  rdfs:comment "Identifier for taxon properties (including the following) of the host" ;
  owl:equivalentProperty dwc:taxonID ;
  rdfs:comment "Automatically populated by TaxaaS. Unsure whether we need taxonID AND taxonConceptID" ;
.
phs:hostTaxonConceptID
  a phs:Host ;
  rdfs:comment "Identifier for taxonomic CONCEPT (not nomenclature) of the host" ;
  owl:equivalentProperty dwc:taxonConceptID ;
  rdfs:comment "Automatically populated by TaxaaS. Unsure whether we need taxonID AND taxonConceptID" ;
.
phs:hostCommonName
  a phs:Host ;
  rdfs:comment "The vernacular (common) name for the host" ;
  owl:equivalentProperty dwc:vernacularName ;
  rdfs:comment "I'd prefer to use hostVernacularName and then do a 'common sameas vernacular'" ;
.
phs:hostScientificName
  a phs:Host ;
  owl:equivalentProperty dwc:scientificName ;
  rdfs:comment "The scientific name of the host" ;
  rdfs:comment "I changed this from taxonName to align with DwC'" ;
.
# Other properties such as rank, parent taxon can be inferred from TaxaaS.
#
#
#ProgramName
#OrganisationName
#samplingProtocol
#samplingProtocolID
#ActivityDescription
#activityClass
#nonTargetPresent
#nonTargetName
#comments
#sampleType
#
## Substrate
#
#Substrate_Name
#
#NonTaxaSubstrateID
#Substrate_OccurrenceID
#Substrate_datasetName
#Substrate_recordNumber
#Substrate_Quantity
#Substrate_QuantityType
#Substrate_RiskCharacters
#
## Darwin Core terms
#dwc:datasetID
#dwc:datasetName
#dwc:institutionCode
#dwc:basisOfRecord
#dwc:modified
#dwc:municipality
#dwc:locality
#dwc:locationID
#dwc:georeferenceSources
#dwc:georeferencedDate
#dwc:geodeticDatum
#dwc:decimalLatitude
#dwc:decimalLongitude
#dwc:footprintWKT
#dwc:footprintSRS
#dwc:coordinateUncertaintyInMeters
#dwc:GeographyLevelID
#dwc:higherGeographyID
#dwc:higherGeography
#dwc:stateProvince
#dwc:eventDate
#dwc:eventEndDate
#dwc:eventID
#dwc:fieldNumber
#dwc:sampleSizeUnit
#dwc:sampleSizeValue
#dwc:scientificName
#dwc:taxonID
#dwc:higherClassification
#dwc:occurrenceStatus
#dwc:occurrenceID
#dwc:recordedBy
#dwc:recordNumber
#dwc:catalogNumber
#dwc:lifeStage
#dwc:reproductiveCondition
#dwc:behavior
#dwc:organismQuantity
#dwc:organismQuantityType
#dwc:occurrenceRemarks
#dwc:identificationID
#dwc:identificationQualifier
#dwc:IdentificationMethod
#dwc:IdentificationResult
#dwc:dateIdentified
#dwc:identifiedBy
