# baseURI: https://linked.data.gov.au/def/phs/voc/inspection-methods
# imports: https://linked.data.gov.au/def/phs
# prefix: inspect

@prefix : <https://linked.data.gov.au/def/phs/voc/inspection-methods/> .
@prefix dcterms: <http://purl.org/dc/terms/> .
@prefix inspect: <https://linked.data.gov.au/def/phs/voc/inspection-methods> .
@prefix owl: <http://www.w3.org/2002/07/owl#> .
@prefix phs: <https://linked.data.gov.au/def/phs#> .
@prefix rdf: <http://www.w3.org/1999/02/22-rdf-syntax-ns#> .
@prefix rdfs: <http://www.w3.org/2000/01/rdf-schema#> .
@prefix sdo: <https://schema.org/> .
@prefix skos: <http://www.w3.org/2004/02/skos/core#> .
@prefix taxaas: <https://uat-ag-bie.oztaxa.com/ws/taxon/> .
@prefix tpg: <https://linked.data.gov.au/def/phs/voc/tpg/> .
@prefix traps: <https://linked.data.gov.au/def/phs/voc/traps/> .
@prefix xsd: <http://www.w3.org/2001/XMLSchema#> .

<http://orcid.org/0000-0002-8742-7730>
  a owl:NamedIndividual ;
  a sdo:Person ;
  sdo:affiliation <https://surroundaustralia.com> ;
  sdo:email <mailto:nicholas.car@surroundaustralia.com> ;
  sdo:jobTitle "Data Systems Architect" ;
  sdo:name "Nicholas J. Car" ;
.
<https://linked.data.gov.au/def/phs/voc/inspection-methods>
  a owl:Ontology ;
  a skos:ConceptScheme ;
  dcterms:contributor <http://orcid.org/0000-0002-8742-7730> ;
  dcterms:created "2020-05-22"^^xsd:date ;
  dcterms:creator <https://orcid.org/0000-0003-3357-2307> ;
  dcterms:modified "2020-05-22"^^xsd:date ;
  dcterms:publisher <https://linked.data.gov.au/org/dawe> ;
  rdfs:comment "Inspection methods are distinguished from identification methods or diagnostic methods by considering where the action is carried out. If it is in the field, then it is an inspection method. The other methods are performed in a laboatory setting. Sometimes there is overlap between these distinctions, such as when simple 'diagnostic' actions are carried out in the field." ;
  owl:imports <https://linked.data.gov.au/def/phs> ;
  owl:versionIRI <https://linked.data.gov.au/def/phs/voc/obsMethods/1.0> ;
  skos:definition "Methods used to perform surveillance for plant pests"@en ;
  skos:hasTopConcept :beating-tray ;
  skos:hasTopConcept :brush-and-vacuum ;
  skos:hasTopConcept :isolation-from-vector ;
  skos:hasTopConcept :sweep-netting ;
  skos:hasTopConcept :tissue-sampling ;
  skos:hasTopConcept :trapping ;
  skos:hasTopConcept :visual ;
  skos:prefLabel "Inspection Method Types"@en ;
.
:beating-tray
  a skos:Concept ;
  a phs:InspectionMethodType ;
  skos:definition "A tray is held under a branch or shrub and the plant is beaten to dislodge insects, which fall onto the tray."@en ;
  skos:inScheme <https://linked.data.gov.au/def/phs/voc/inspection-methods> ;
  skos:prefLabel "Beating tray"@en ;
  skos:topConceptOf <https://linked.data.gov.au/def/phs/voc/inspection-methods> ;
  phs:detectsPest tpg:bmsb ;
  phs:detectsPest tpg:xylella-vectors ;
.
:brush-and-vacuum
  a skos:Concept ;
  a phs:InspectionMethodType ;
  skos:definition "Areas are vacuumed and the collected debris is inspected for target pests"@en ;
  skos:inScheme <https://linked.data.gov.au/def/phs/voc/inspection-methods> ;
  skos:prefLabel "Brush and vacuum"@en ;
  skos:topConceptOf <https://linked.data.gov.au/def/phs/voc/inspection-methods> ;
  phs:detectsPest tpg:khapra-beetle ;
.
:isolation-from-vector
  a skos:Concept ;
  a phs:InspectionMethodType ;
  skos:definition "After a vector (usually an insect) is captured, it is treated in such a way as to expose the target pest. Procedures vary according to the circumstances. As an example, in 'sugar shaking', bees (the vector) are placed in a plastic bag with castor sugar and shaken. The surviving bees are released. The sugar is dissolved and filtered, leaving mites on the filter paper."@en ;
  skos:inScheme <https://linked.data.gov.au/def/phs/voc/inspection-methods> ;
  skos:prefLabel "Isolation from vector"@en ;
  skos:topConceptOf <https://linked.data.gov.au/def/phs/voc/inspection-methods> ;
  phs:detectsPest tpg:pine-wilt-nematode ;
.
:sweep-netting
  a skos:Concept ;
  a phs:InspectionMethodType ;
  skos:definition "A light net is dragged across the tops of plants or directly aimed at flying insects. The archetypal method for collecting insects."@en ;
  skos:inScheme <https://linked.data.gov.au/def/phs/voc/inspection-methods> ;
  skos:prefLabel "Sweep netting"@en ;
  skos:topConceptOf <https://linked.data.gov.au/def/phs/voc/inspection-methods> ;
  phs:detectsPest tpg:bmsb ;
  phs:detectsPest tpg:khapra-beetle ;
  phs:detectsPest tpg:xylella-vectors ;
.
:tissue-sampling
  a skos:Concept ;
  a phs:InspectionMethodType ;
  skos:definition "This might better be described as a diagnostic method."@en ;
  skos:inScheme <https://linked.data.gov.au/def/phs/voc/inspection-methods> ;
  skos:prefLabel "Tissue sampling"@en ;
  skos:topConceptOf <https://linked.data.gov.au/def/phs/voc/inspection-methods> ;
  phs:detectsPest tpg:pine-wilt-nematode ;
.
:trapping
  a skos:Concept ;
  a phs:InspectionMethodType ;
  skos:definition "A trap is placed in a likely location and revisited after some period, which can vary from hours to weeks"@en ;
  skos:inScheme <https://linked.data.gov.au/def/phs/voc/inspection-methods> ;
  skos:prefLabel "Trapping"@en ;
  skos:topConceptOf <https://linked.data.gov.au/def/phs/voc/inspection-methods> ;
  phs:detectsPest tpg:ants ;
  phs:detectsPest tpg:bmsb ;
  phs:detectsPest tpg:citrus-canker ;
  phs:detectsPest tpg:fall-and-southern-armyworm ;
  phs:detectsPest tpg:fire-blight ;
  phs:detectsPest tpg:khapra-beetle ;
  phs:detectsPest tpg:saywer-beetle ;
  phs:detectsPest tpg:snails ;
  phs:detectsPest tpg:xylella-vectors ;
.
:visual
  a skos:Concept ;
  a phs:InspectionMethodType ;
  skos:definition ""@en ;
  skos:inScheme <https://linked.data.gov.au/def/phs/voc/inspection-methods> ;
  skos:prefLabel "Visual"@en ;
  skos:topConceptOf <https://linked.data.gov.au/def/phs/voc/inspection-methods> ;
  phs:detectsPest tpg:anaplophora ;
  phs:detectsPest tpg:ants ;
  phs:detectsPest tpg:bmsb ;
  phs:detectsPest tpg:citrus-canker ;
  phs:detectsPest tpg:fall-and-southern-armyworm ;
  phs:detectsPest tpg:fire-blight ;
  phs:detectsPest tpg:fruit-fly ;
  phs:detectsPest tpg:gypsy-moth ;
  phs:detectsPest tpg:hlb ;
  phs:detectsPest tpg:hlb-vectors ;
  phs:detectsPest tpg:khapra-beetle ;
  phs:detectsPest tpg:pine-wilt-nematode ;
  phs:detectsPest tpg:saywer-beetle ;
  phs:detectsPest tpg:snails ;
  phs:detectsPest tpg:xylella-fastidiosa ;
  phs:detectsPest tpg:xylella-vectors ;
.
<https://linked.data.gov.au/org/dawe>
  a owl:NamedIndividual ;
  a sdo:Organization ;
  sdo:name "Department of Agriculture, Water and the Environment" ;
  sdo:url <https://www.awe.gov.au/> ;
.
<https://orcid.org/0000-0003-3357-2307>
  a owl:NamedIndividual ;
  a sdo:Person ;
  sdo:affiliation <https://linked.data.gov.au/org/dawe> ;
  sdo:email <mailto:stephen.pratt@awe.gov.au> ;
  sdo:jobTitle "Project Manager: Implementation of Plant Health Surveillance Data Store" ;
  sdo:name "Stephen J. Pratt" ;
.
