#
@prefix : <https://linked.data.gov.au/def/phs/voc/inspection-methods/> .
@prefix inspect: <https://linked.data.gov.au/def/phs/voc/inspection-methods> .
@prefix dcterms: <http://purl.org/dc/terms/> .
@prefix rdfs: <http://www.w3.org/2000/01/rdf-schema#> .
@prefix sdo: <https://schema.org/> .
@prefix skos: <http://www.w3.org/2004/02/skos/core#> .
@prefix owl: <http://www.w3.org/2002/07/owl#> .
@prefix taxaas: <https://uat-ag-bie.oztaxa.com/ws/taxon/> .
@prefix phs: <https://linked.data.gov.au/def/phs#> .
@prefix tpg: <https://linked.data.gov.au/def/phs/voc/tpg/> .
@prefix traps: <https://linked.data.gov.au/def/phs/voc/traps/> .
@prefix xsd: <http://www.w3.org/2001/XMLSchema#> .

inspect:
    a owl:Ontology , skos:ConceptScheme ;
    dcterms:contributor <http://orcid.org/0000-0002-8742-7730> ;
    dcterms:created "2020-05-22"^^xsd:date ;
    dcterms:creator phs:stephen ;
    dcterms:modified "2020-05-22"^^xsd:date ;
    dcterms:publisher <https://linked.data.gov.au/org/dawe> ;
    skos:definition "Methods used to perform surveillance for plant pests"@en ;
    rdfs:comment "Inspection methods are distinguished from identification methods or diagnostic methods by considering where the action is carried out. If it is in the field, then it is an inspection method. The other methods are performed in a laboatory setting. Sometimes there is overlap between these distinctions, such as when simple 'diagnostic' actions are carried out in the field." ;
    skos:prefLabel "Inspection Method Types"@en ;
    owl:versionIRI <https://linked.data.gov.au/def/phs/voc/obsMethods/1.0> ;
    skos:hasTopConcept 
        :beating-tray , 
        :brush-and-vacuum ,
        :isolation-from-vector ,
        :sweep-netting ,
        :tissue-sampling ,
        :trapping ,
        :visual ;
.

:beating-tray
    a skos:Concept , phs:InspectionMethodType ;
    skos:prefLabel "Beating tray"@en ;    
    skos:definition "A tray is held under a branch or shrub and the plant is beaten to dislodge insects, which fall onto the tray."@en ;
    skos:inScheme inspect: ;
    skos:topConceptOf inspect:;
    phs:detectsPest tpg:bmsb , tpg:xylella-vectors ;  
.

:brush-and-vacuum
    a skos:Concept , phs:InspectionMethodType ;
    skos:prefLabel "Brush and vacuum"@en ;    
    skos:definition "Areas are vacuumed and the collected debris is inspected for target pests"@en ;
    skos:inScheme inspect: ;
    skos:topConceptOf inspect:;
    phs:detectsPest tpg:khapra-beetle ;  
.

:isolation-from-vector
    a skos:Concept , phs:InspectionMethodType ;
    skos:prefLabel "Isolation from vector"@en ;    
    skos:definition "After a vector (usually an insect) is captured, it is treated in such a way as to expose the target pest. Procedures vary according to the circumstances. As an example, in 'sugar shaking', bees (the vector) are placed in a plastic bag with castor sugar and shaken. The surviving bees are released. The sugar is dissolved and filtered, leaving mites on the filter paper."@en ;
    skos:inScheme inspect: ;
    skos:topConceptOf inspect:;
    phs:detectsPest tpg:pine-wilt-nematode ;  
.

:sweep-netting
    a skos:Concept , phs:InspectionMethodType ;
    skos:prefLabel "Sweep netting"@en ;    
    skos:definition "A light net is dragged across the tops of plants or directly aimed at flying insects. The archetypal method for collecting insects."@en ;
    skos:inScheme inspect: ;
    skos:topConceptOf inspect:;
    phs:detectsPest 
        tpg:bmsb ,
        tpg:khapra-beetle ,
        tpg:xylella-vectors ;  
.

:tissue-sampling
    a skos:Concept , phs:InspectionMethodType ;
    skos:prefLabel "Tissue sampling"@en ;    
    skos:definition "This might better be described as a diagnostic method."@en ;
    skos:inScheme inspect: ;
    skos:topConceptOf inspect:;
    phs:detectsPest tpg:pine-wilt-nematode ;  
.

:trapping
    a skos:Concept , phs:InspectionMethodType ;
    skos:prefLabel "Trapping"@en ;    
    skos:definition "A trap is placed in a likely location and revisited after some period, which can vary from hours to weeks"@en ;
    skos:inScheme inspect: ;
    skos:topConceptOf inspect: ;
    phs:detectsPest 
        tpg:fall-and-southern-armyworm , 
        tpg:bmsb , 
        tpg:citrus-canker , 
        tpg:fire-blight , 
        tpg:khapra-beetle , 
        tpg:saywer-beetle , 
        tpg:xylella-vectors , 
        tpg:ants ,
     tpg:snails ;  
.

:visual
    a skos:Concept , phs:InspectionMethodType ;
    skos:prefLabel "Visual"@en ;    
    skos:definition ""@en ;
    skos:inScheme inspect: ;
    skos:topConceptOf inspect: ;
    phs:detectsPest 
        tpg:anaplophora , 
        tpg:fall-and-southern-armyworm , 
        tpg:bmsb , 
        tpg:citrus-canker , 
        tpg:fire-blight , 
        tpg:gypsy-moth , 
        tpg:fruit-fly , 
        tpg:hlb , 
        tpg:hlb-vectors , 
        tpg:khapra-beetle , 
        tpg:saywer-beetle , 
        tpg:pine-wilt-nematode , 
        tpg:xylella-fastidiosa , 
        tpg:xylella-vectors , 
        tpg:ants , 
        tpg:snails ;  
.

<https://linked.data.gov.au/org/dawe> 
    a owl:NamedIndividual , sdo:Organization ;
    sdo:name "Department of Agriculture, Water and the Environment" ;
    sdo:url <https://www.awe.gov.au/> .

<http://orcid.org/0000-0002-8742-7730> 
    a owl:NamedIndividual , sdo:Person ;
    sdo:affiliation <https://surroundaustralia.com> ;
    sdo:email <mailto:nicholas.car@surroundaustralia.com> ;
    sdo:jobTitle "Data Systems Architect" ;
    sdo:name "Nicholas J. Car" .

phs:stephen a owl:NamedIndividual , sdo:Person ;
         sdo:affiliation <https://linked.data.gov.au/org/dawe> ;
         sdo:email <mailto:stephen.pratt@awe.gov.au> ;
         sdo:jobTitle "Project Manager: Implementation of Plant Health Surveillance Data Store" ;
         sdo:name "Stephen J. Pratt" .
