#
@prefix : <https://linked.data.gov.au/def/phs/voc/occstatuses/> .
@prefix occstatuses: <https://linked.data.gov.au/def/phs/voc/occstatuses> .
@prefix phs: <https://linked.data.gov.au/def/phs#> .
@prefix tpg: <https://linked.data.gov.au/def/phs/voc/tpg/> .
@prefix dcterms: <http://purl.org/dc/terms/> .
@prefix rdfs: <http://www.w3.org/2000/01/rdf-schema#> .
@prefix sdo: <https://schema.org/> .
@prefix skos: <http://www.w3.org/2004/02/skos/core#> .
@prefix owl: <http://www.w3.org/2002/07/owl#> .
@prefix taxaas: <https://uat-ag-bie.oztaxa.com/ws/taxon/> .
@prefix xsd: <http://www.w3.org/2001/XMLSchema#> .

occstatuses:
    a owl:Ontology , skos:ConceptScheme ;
    dcterms:contributor <http://orcid.org/0000-0002-8742-7730> ;
    dcterms:created "2021-05-14"^^xsd:date ;
    dcterms:creator <https://orcid.org/0000-0003-3357-2307> ;
    dcterms:modified "2021-05-14"^^xsd:date ;
    dcterms:publisher <https://linked.data.gov.au/org/dawe> ;
    skos:definition "Statuses that apply to the occurrence of target pests with respect to a single observation"@en ;
    skos:prefLabel "Occurrence Statuses of target pests"@en ;
    rdfs:comment "These occurrence statuses apply only to the observation within which they were applied. They do not relate to distribituions or prevalences of target pests. e.g. A pest may indeed by present even though it was not detected by a given observation." ;
    owl:versionIRI <https://linked.data.gov.au/def/phs/voc/occstatuses/1.0> ;
    skos:hasTopConcept
        :present ;
        :absent ;
        :pending ;
        :inconclusive ;
.

:present
    a skos:Concept , phs:OccurrenceStatus
    skos:prefLabel "Present"@en ;
    skos:definition "The target pest group was detected by the observation event"@en ;
    skos:inScheme occstatuses ;
    skos:topConceptOf occstatuses ;

:absent
    a skos:Concept , phs:OccurrenceStatus
    skos:prefLabel "Absent"@en ;
    skos:definition "The target pest group was not detected by the observation event"@en ;
    skos:inScheme occstatuses ;
    skos:topConceptOf occstatuses ;

:pending
    a skos:Concept , phs:OccurrenceStatus
    skos:prefLabel "Pending"@en ;
    skos:definition "Diagnostic procedures are not yet complete"@en ;
    rdfs:comment "This status implies that the occurence status of the observation event will be updated once the diagnostic work is complete"@en ;
    skos:inScheme occstatuses ;
    skos:topConceptOf occstatuses ;

:inconclusive
    a skos:Concept , phs:OccurrenceStatus
    skos:prefLabel "Inconclusive"@en ;
    skos:definition "The identity of specimens was not able to be determined"@en ;
    rdfs:comment "This status may change if subsequent diagnostic work is able to identify the specimen, but it may remain as 'Inconclusive if resources are not available to carry out the work, required specialist skills are not available, the specimen is degraded, or the taxonomy surrounding the specimen is uncertain."@en ;
    skos:inScheme occstatuses ;
    skos:topConceptOf occstatuses ;
.


